defined signatures, models, and specs in Coq
git-svn-id: svn+ssh://svn.kestrel.edu/Specware/trunk@9049 7b97033b-253e-4a5c-9b07-e25f9089a9fd

Provers/ToCoq/Spec_Inductive_New.v
@@ -1,34 +1,145 @@
 
-(*** An approach to representing Specs with inductive types ***)
+(*** An approach to representing Models with inductive types ***)
 
-(* A glorified record type *)
-Inductive SpecType : Type :=
-| SpecType_Nil : SpecType
-| SpecType_Cons (A : Type) : (A -> SpecType) -> SpecType
+Require Import String.
+Require Import List.
+
+(* A signature is a glorified record type *)
+Inductive Sig : list string -> Type :=
+| Sig_Nil : Sig nil
+| Sig_Cons f (A : Type) flds : ~In f flds -> (A -> Sig flds) -> Sig (f :: flds)
 .
 
-(* An element of a SpecType *)
-Inductive SpecElem : SpecType -> Type :=
-| SpecElem_Nil : SpecElem SpecType_Nil
-| SpecElem_Cons A B a : SpecElem (B a) -> SpecElem (SpecType_Cons A B)
+(* A Model is an element of the record type denoted by a Sig *)
+Inductive Model : forall {flds}, Sig flds -> Type :=
+| Model_Nil : Model Sig_Nil
+| Model_Cons f A a flds nodup sig  :
+    Model (flds:=flds) (sig a) ->
+    Model (Sig_Cons f A flds nodup sig)
 .
 
-(* A partial element of a SpecType *)
-Inductive PartialElem : SpecType -> Type :=
-| Part_Nil : PartialElem SpecType_Nil
-| Part_ConsNone A B : (forall a, PartialElem (B a)) -> PartialElem (SpecType_Cons A B)
-| Part_ConsSome A B a : PartialElem (B a) -> PartialElem (SpecType_Cons A B)
+(* A Spec is a partial Model of a Sig *)
+Inductive Spec : forall {flds}, Sig flds -> Type :=
+| Spec_Nil : Spec Sig_Nil
+| Spec_ConsNone f A flds nodup sig  :
+    (forall a, Spec (flds:=flds) (sig a)) -> Spec (Sig_Cons f A flds nodup sig)
+| Spec_ConsSome f A a flds nodup sig  :
+    Spec (flds:=flds) (sig a) ->
+    Spec (Sig_Cons f A flds nodup sig)
 .
 
-(* A partial element can "complete" to an element *)
-Inductive CompletesTo : forall T, PartialElem T -> SpecElem T -> Prop :=
-| CompletesTo_Nil : CompletesTo _ Part_Nil SpecElem_Nil
-| CompletesTo_ConsNone A B a pelem elem :
-    CompletesTo (B a) (pelem a) elem ->
-    CompletesTo (SpecType_Cons A B) (Part_ConsNone A B pelem)
-                (SpecElem_Cons A B a elem)
-| CompletesTo_ConsSome A B a pelem elem :
-    CompletesTo (B a) pelem elem ->
-    CompletesTo (SpecType_Cons A B) (Part_ConsSome A B a pelem)
-                (SpecElem_Cons A B a elem)
+(* A model of a Spec supplies missing fields but is otherwise equal *)
+Inductive IsModel : forall {flds sig}, Spec (flds:=flds) sig -> Model (flds:=flds) sig -> Prop :=
+| IsModel_Nil : IsModel Spec_Nil Model_Nil
+| IsModel_ConsNone f A a flds nodup sig spec model :
+    IsModel (spec a) model ->
+    IsModel (Spec_ConsNone f A flds nodup sig spec)
+            (Model_Cons f A a flds nodup sig model)
+| IsModel_ConsSome f A a flds nodup sig spec model :
+    IsModel spec model ->
+    IsModel (Spec_ConsSome f A a flds nodup sig spec)
+            (Model_Cons f A a flds nodup sig model)
 .
+
+(* FIXME: write prove_ismodel tactic *)
+
+(* helper function for eliminating ors *)
+Definition or_proj_r A B : ~A -> A \/ B -> B.
+  intros not_A or; destruct or.
+  elimtype False; apply not_A; assumption.
+  assumption.
+Qed.
+
+Definition or_proj_l A B : ~B -> A \/ B -> A.
+  intros not_B or; destruct or.
+  assumption.
+  elimtype False; apply not_B; assumption.
+Qed.
+
+
+(* Proof that field f is associated with type A in signature, where A
+   quantifies over all types before f in the Sig *)
+Inductive SigElem (f : string) : Type -> forall {flds}, Sig flds -> Prop :=
+| SigElem_Base A flds nodup sig :
+    SigElem f A (Sig_Cons f A flds nodup sig)
+| SigElem_Cons f' A' A flds nodup sig :
+    (forall (a:A'), SigElem f (A a) (sig a)) ->
+    SigElem f (forall (a:A'), A a) (Sig_Cons f' A' flds nodup sig)
+.
+
+(* Proof that field f is associated with non-dependent type A in signature *)
+Inductive SigElem_nondep (f : string) A : forall {flds}, Sig flds -> Prop :=
+| SigElem_nondep_Base flds nodup sig :
+    SigElem_nondep f A (Sig_Cons f A flds nodup sig)
+| SigElem_nondep_Cons f' A' flds nodup sig :
+    (forall a, SigElem_nondep f A (sig a)) ->
+    SigElem_nondep f A (Sig_Cons f' A' flds nodup sig)
+.
+
+(* Proof that field f is associated with element a of type A in model *)
+Inductive ModelElem (f : string) A (a:A) : forall {flds sig}, Model (flds:=flds) sig -> Prop :=
+| ModelElem_Base flds nodup sig model :
+    ModelElem f A a (Model_Cons f A a flds nodup sig model)
+| ModelElem_Cons f' A' a' flds nodup sig model :
+    ModelElem f A a model ->
+    ModelElem f A a (Model_Cons f' A' a' flds nodup sig model)
+.
+
+(* Projecting an element out of a Model *)
+Fixpoint modelProj {flds sig} (model : Model (flds:=flds) sig) :
+  forall f, In f flds -> { A : Type & A } :=
+  match model in Model (flds:=flds) sig
+        return forall f, In f flds -> { A : Type & A }
+  with
+    | Model_Nil => fun f in_nil => False_rect _ in_nil
+    | Model_Cons f' A a _ _ _ model =>
+      fun f in_pf =>
+        match string_dec f' f with
+            | left _ => existT id A a
+            | right neq =>
+              modelProj model f (or_proj_r _ _ neq in_pf)
+        end
+  end.
+
+(* Correctness of modelProj: always returns a ModelElem *)
+Lemma modelProj_correct flds sig (model : Model (flds:=flds) sig) f in_pf :
+  ModelElem f (projT1 (modelProj model f in_pf))
+            (projT2 (modelProj model f in_pf))
+            model.
+  revert f in_pf; induction model; intros.
+  elimtype False; apply in_pf.
+  unfold modelProj; fold (modelProj (flds:=flds) (sig:=sig a)).
+  destruct (string_dec f f0).
+  rewrite <- e; apply ModelElem_Base.
+  apply ModelElem_Cons.
+  apply IHmodel.
+Qed.
+
+
+(* Models can be translated by "unapplying" a function on fields *)
+(* FIXME: can only translate when we know the projected type is preserved
+Fixpoint modelXlate {flds1 sig1} :
+  ({f | In f flds1} -> {f | In f flds2}) ->
+  forall {flds2 sig2},
+    Model (flds:=flds2) sig2 ->
+    Model (flds:=flds1) sig1 :=
+  match sig1 in Sig flds1
+        return
+        ({f | In f flds1} -> {f | In f flds2}) ->
+        forall {flds2 sig2},
+          Model (flds:=flds2) sig2 ->
+          Model (flds:=flds1) sig1
+  with
+    | Sig_Nil => Model_Nil
+    | Sig_Cons f A flds nodup sig =>
+      fun xlate flds2 sig2 model2 =>
+        Model_Cons f A 
+*)
+
+Inductive ModelXlates {flds2 sig2} (model2 : Model (flds:=flds2) sig2) :
+  forall {flds1 sig1},
+    Model (flds:=flds1) sig1 ->
+    ({f | In f flds1} -> {f | In f flds2}) -> Prop :=
+| ModelXlates_Nil : ModelXlates model2
+
+(* A morphism maps a spec to one with a subset of the models *)
